backend/Linearizeproof.v
@@ -251,10 +251,6 @@ Proof.
   destruct a; simpl in UNIQ; tauto.
 Qed.
 
-(** [CompCertX:test-compcert-protect-stack-arg] We also parameterize over a way to mark blocks writable. *)
-Section WITHWRITABLEBLOCK.
-Context `{Hwritable_block: WritableBlock}.
-
 (** Correctness of the [starts_with] test. *)
 
 Lemma starts_with_correct:
@@ -560,6 +556,8 @@ Definition measure (S: LTL.state) : nat :=
   | _ => 0%nat
   end.
 
+Section WITHINITLS.
+
 Variable init_ls: locset.
 
 Remark match_parent_locset:
@@ -629,9 +627,6 @@ Proof.
   apply plus_one. econstructor.
   instantiate (1 := a). rewrite <- H; apply eval_addressing_preserved.
   exact symbols_preserved. eauto. eauto.
-  {
-    intros. eapply writable_block_genv_next; [ | eauto ]. apply genv_next_preserved.
-  }
   econstructor; eauto.
 
   (* Lcall *)
@@ -655,9 +650,7 @@ Proof.
   left; econstructor; split. simpl.
   apply plus_one. eapply exec_Lbuiltin; eauto.
   eapply eval_builtin_args_preserved with (ge1 := ge); eauto. exact symbols_preserved.
-  eapply external_call_writable_block_weak.
   eapply external_call_symbols_preserved; eauto. apply senv_preserved.
-  apply writable_block_genv_next. apply genv_next_preserved.
   econstructor; eauto.
 
   (* Lbranch *)
@@ -714,9 +707,7 @@ Proof.
   (* external function *)
   monadInv H8. left; econstructor; split.
   apply plus_one. eapply exec_function_external; eauto.
-  eapply external_call_writable_block_weak.
   eapply external_call_symbols_preserved; eauto. apply senv_preserved.
-  apply writable_block_genv_next. apply genv_next_preserved.
   econstructor; eauto.
 
   (* return *)
@@ -725,8 +716,6 @@ Proof.
   apply plus_one. econstructor.
   econstructor; eauto.
 Qed.
-
-End WITHWRITABLEBLOCK.
 
 Lemma transf_initial_states:
   forall st1, LTL.initial_state prog st1 ->
@@ -749,9 +738,7 @@ Proof.
   intros. inv H0. inv H. inv H5. econstructor; eauto.
 Qed.
 
-(** [CompCertX:test-compcert-protect-stack-arg] For whole programs, all blocks are writable. *)
-Local Existing Instance writable_block_always_ops.
-Local Existing Instance writable_block_always.
+End WITHINITLS.
 
 Theorem transf_program_correct:
   forward_simulation (LTL.semantics prog) (Linear.semantics tprog).
