backend/Tunnelingproof.v
@@ -266,9 +266,7 @@ Definition measure (st: state) : nat :=
   | Returnstate s ls m => 0%nat
   end.
 
-(** [CompCertX:test-compcert-protect-stack-arg] We also parameterize over a way to mark blocks writable. *)
-Section WITHWRITABLEBLOCK.
-Context `{Hwritable_block: WritableBlock}.
+Section WITHINITLS.
 
 Variable init_ls: locset.
 
@@ -328,9 +326,6 @@ Proof.
   eapply exec_Lstore with (a0 := a).
   rewrite <- H. apply eval_addressing_preserved. exact symbols_preserved.
   eauto. eauto.
-  { (* writable block *)
-    intros. eapply writable_block_genv_next; [ | eauto ]. apply genv_next_preserved.
-  }
   econstructor; eauto.
   (* Lcall *)
   left; simpl; econstructor; split.
@@ -352,9 +347,7 @@ Proof.
   left; simpl; econstructor; split.
   eapply exec_Lbuiltin; eauto.
   eapply eval_builtin_args_preserved with (ge1 := ge); eauto. exact symbols_preserved.
-  eapply external_call_writable_block_weak.
   eapply external_call_symbols_preserved. apply senv_preserved. eauto.
-  apply writable_block_genv_next. apply genv_next_preserved.
   econstructor; eauto.
 
   (* Lbranch (preserved) *)
@@ -385,9 +378,7 @@ Proof.
   (* external function *)
   left; simpl; econstructor; split.
   eapply exec_function_external; eauto.
-  eapply external_call_writable_block_weak.
   eapply external_call_symbols_preserved; eauto. apply senv_preserved.
-  apply writable_block_genv_next. apply genv_next_preserved.
   simpl. econstructor; eauto.
   (* return *)
   inv H3. inv H1.
@@ -396,7 +387,7 @@ Proof.
   constructor; auto.
 Qed.
 
-End WITHWRITABLEBLOCK.
+End WITHINITLS.
 
 Lemma transf_initial_states:
   forall st1, initial_state prog st1 ->
@@ -419,10 +410,6 @@ Lemma transf_final_states:
 Proof.
   intros. inv H0. inv H. inv H5. econstructor; eauto.
 Qed.
-
-(** [CompCertX:test-compcert-protect-stack-arg] For whole programs, all blocks are writable. *)
-Local Existing Instance writable_block_always_ops.
-Local Existing Instance writable_block_always.
 
 Theorem transf_program_correct:
   forward_simulation (LTL.semantics prog) (LTL.semantics tprog).
