cfrontend/ClightBigstep.v
@@ -34,9 +34,6 @@ Context `{external_calls_prf: ExternalCalls}.
 
 Section BIGSTEP.
 
-(** [CompCertX:test-compcert-protect-stack-arg] We also parameterize over a way to mark blocks writable. *)
-Context `{writable_block_ops: WritableBlockOps}.
-
 Variable ge: genv.
 
 (** ** Big-step semantics for terminating statements and functions *)
@@ -108,7 +105,7 @@ Inductive exec_stmt: env -> temp_env -> mem -> statement -> trace -> temp_env ->
                 t (set_opttemp optid vres le) m' Out_normal
   | exec_Sbuiltin:   forall e le m optid ef al tyargs vargs t m' vres,
       eval_exprlist ge e le m al tyargs vargs ->
-      external_call ef (writable_block ge) ge vargs m t vres m' ->
+      external_call ef ge vargs m t vres m' ->
       exec_stmt e le m (Sbuiltin optid ef tyargs al)
                 t (set_opttemp optid vres le) m' Out_normal
   | exec_Sseq_1:   forall e le m s1 s2 t1 le1 m1 t2 le2 m2 out,
@@ -178,7 +175,7 @@ with eval_funcall: mem -> fundef -> list val -> trace -> mem -> val -> Prop :=
       Mem.free_list m3 (blocks_of_env ge e) = Some m4 ->
       eval_funcall m (Internal f) vargs t m4 vres
   | eval_funcall_external: forall m ef targs tres cconv vargs t vres m',
-      external_call ef (writable_block ge) ge vargs m t vres m' ->
+      external_call ef ge vargs m t vres m' ->
       eval_funcall m (External ef targs tres cconv) vargs t m' vres.
 
 Scheme exec_stmt_ind2 := Minimality for exec_stmt Sort Prop
@@ -246,9 +243,7 @@ End BIGSTEP.
 
 (** Big-step execution of a whole program.  *)
 
-(** [CompCertX:test-compcert-protect-stack-arg] For whole programs, all blocks are writable. *)
 Section WHOLE_PROGRAM.
-Local Existing Instance writable_block_always_ops.
 
 Variable function_entry: genv -> function -> list val -> mem -> env -> temp_env -> mem -> Prop.
 
@@ -284,9 +279,6 @@ Section BIGSTEP_TO_TRANSITIONS.
 Variable prog: program.
 Let ge : genv := globalenv prog.
 
-Section WITHWRITABLEBLOCK.
-Context `{writable_block_ops: WritableBlockOps}.
-
 Inductive outcome_state_match
        (e: env) (le: temp_env) (m: mem) (f: function) (k: cont): outcome -> state -> Prop :=
   | osm_normal:
@@ -310,6 +302,8 @@ Lemma is_call_cont_call_cont:
 Proof.
   destruct k; simpl; intros; contradiction || auto.
 Qed.
+
+Section WITHFUNCTIONENTRY.
 
 Variable function_entry: genv -> function -> list val -> mem -> env -> temp_env -> mem -> Prop.
 
@@ -581,9 +575,7 @@ Proof.
   traceEq.
 Qed.
 
-End WITHWRITABLEBLOCK.
-
-Local Existing Instance writable_block_always_ops.
+End WITHFUNCTIONENTRY.
 
 Theorem bigstep_semantics_sound:
   bigstep_sound (bigstep_semantics (function_entry1) prog) (semantics1 prog).
